FiniteRing half done

theories/algebra/FiniteRing.ec
@@ -1,5 +1,6 @@
 (* ==================================================================== *)
-require import AllCore List Ring Int IntMin IntDiv RingStruct Finite FinType ZModP.
+require import AllCore List Ring Int IntMin IntDiv RingStruct Finite.
+require import FinType ZModP UnitRing.
 require import Bigalg SubRing RingModule Real RealExp Quotient Counting.
 require (*--*) Subtype.
 (*---*) import StdOrder.IntOrder.
@@ -9,24 +10,25 @@ require (*--*) Subtype.
 abstract theory SubFinite.
   type t, st.
 
-  op p : t -> bool.
-
-  clone import FinType as FT with
+  clone import FinType as TFT with
     type t <= t.
+
+  (*TODO: Pierre-Yves: this is needed because P is a pred in Sub and
+                       must be used as an op in filter.
+                       we need to replace pred by op everywhere in the StdLib*)
+  op P : t -> bool.
 
   clone import Subtype as Sub with
     type T  <= t ,
     type sT <= st,
-    pred P  <= p.
+    pred P  <= P.
 
   import Sub.
 
-  op senum = map insubd (filter p enum).
-
   clone import FinType as SFT with
     type t  <= st,
-    op enum <= senum
-    proof *.
+    op enum <= map insubd (filter P enum)
+  proof *.
 
   realize enum_spec.
   proof.
@@ -41,766 +43,713 @@ end SubFinite.
 
 (* ==================================================================== *)
 abstract theory FiniteZModule.
-  type t.
+  clone include ZModuleStruct.
 
-  clone import ZModule as ZMod with
+  clone import FinType.FinType as FT with
     type t <= t.
 
-  clone import FinType.FinType as FinType with
-    type t <= t.
+  theory FZMod.
+    import RL ZModStr FT.
+
+    lemma gt0_order x :
+      0 < order x.
+    proof.
+      case/ler_eqVlt: (ge0_order x) => // /eq_sym /order0P => inj_intmul.
+      by have //: false; move: inj_intmul => /=; apply/not_injective_int.
+    qed.
+  
+    import StdBigop.Bigint.
+  
+    lemma dvd_order_card x :
+      order x %| FT.card.
+    proof.
+      have /(_ FT.enum):
+        forall s , exists c ,
+          uniq c /\
+          (forall y z , y \in c => z \in c => eqv_orbit x y z => y = z) /\
+          (mem s <= mem (flatten (map (fun y => map (RL.(+) y) (orbit_list x)) c))).
+      + elim => [|y s [c] IHs]; [by exists [] => /=; rewrite flatten_nil|].
+        move: IHs; pose l:= flatten _; case (y \in l) => [mem_y|Nmem_y];
+        move => [uniq_ [forall_ mem_incl]].
+        - by exists c; split => //; split => // z /= [->>|]; [apply/mem_y|apply/mem_incl].
+        exists (y :: c); do!split => // [|z t|z] /=; [|move => [->>|mem_z] [->>|mem_t] //|].
+        - move: Nmem_y; apply/contra; rewrite /l => {l mem_incl} mem_y; apply/flatten_mapP.
+          exists y; split => //=; apply/mapP; exists zeror; rewrite addr0 /=.
+          by apply/orbit_listP; rewrite ?gt0_order // orbit0.
+        - rewrite /eqv_orbit orbit_listP ?gt0_order //; move: Nmem_y; rewrite /l -flatten_mapP.
+          rewrite negb_exists => /= /(_ t); rewrite mem_t /= mapP negb_exists /= => /(_ (y - t)).
+          by rewrite addrA addrAC subrr /= add0r.
+        - rewrite eqv_orbit_sym /eqv_orbit orbit_listP ?gt0_order //.
+          move: Nmem_y; rewrite /l -flatten_mapP.
+          rewrite negb_exists => /= /(_ z); rewrite mem_z /= mapP negb_exists /= => /(_ (y - z)).
+          by rewrite addrA addrAC subrr /= add0r.
+        - by apply/forall_.
+        rewrite flatten_cons -/l mem_cat; case => [->>|?]; [left|by right; apply/mem_incl].
+        apply/mapP; exists zeror; rewrite addr0 /=.
+        by apply/orbit_listP; rewrite ?gt0_order // orbit0.
+      case => c; pose l:= flatten _; move => [uniq_ [forall_ mem_incl]].
+      rewrite /card (perm_eq_size _ l).
+      + apply/uniq_perm_eq; [by apply/FT.enum_uniq| |]; last first.
+        - by move => ?; split; [apply/mem_incl|move => _; apply/FT.enumP].
+        rewrite /l => {mem_incl l}; apply/uniq_flatten_map => //.
+        - move => y /=; rewrite map_inj_in_uniq; [by move => ? ? _ _; apply/addrI|].
+          by apply/uniq_orbit_list.
+        move => y z mem_y mem_z /= /hasP [?] [] /mapP [t] [mem_t ->>] /mapP [u] [mem_u].
+        move=> eq_.
+        apply/forall_ => //; move: eq_; rewrite /eqv_orbit addrC -eqr_sub => <-.
+        by apply/orbitB; apply/orbit_listP => //; apply/gt0_order.
+      rewrite /l size_flatten sumzE (BIA.eq_big_seq _ (fun _ => order x)) /=.
+      + move => ? /mapP [?] [+ ->>]; move => /mapP [?] /= [_ ->>].
+        by rewrite size_map size_orbit_list.
+      by rewrite BIA.sumr_const count_predT !size_map intmulz; apply/dvdz_mulr/dvdzz.
+    qed.
+  
+    lemma isgeneratorP g :
+      is_generator g <=> order g = card.
+    proof.
+      rewrite /is_generator -size_orbit_list; split => [orbit_|].
+      + apply/perm_eq_size/uniq_perm_eq; [by apply/uniq_orbit_list|by apply/enum_uniq|].
+        by move => x; rewrite -orbit_listP ?gt0_order // orbit_ enumP.
+      move => eq_ x; move: (uniq_leq_size_perm_eq (orbit_list g) enum).
+      rewrite orbit_listP ?gt0_order // uniq_orbit_list enum_uniq eq_ /card /= => /(_ _).
+      + by move => ? _; apply/enumP.
+      by move/perm_eq_mem => ->; apply/enumP.
+    qed.
+  
+    op eq_order d x = order x = d.
+  
+    lemma few_small_order_exists_generator :
+      (forall d , 0 <= d => d %| card =>
+        size (to_seq (fun x => RL.intmul x d = zeror)) <= d) =>
+      exists g , is_generator g.
+    proof.
+      move => forall_.
+      have: forall d , 0 <= d => d %| card => size (to_seq (eq_order d)) <= phi (d).
+      + move => d /ler_eqVlt [<<- _|lt0d dvdd_]; [rewrite phi_eq0 //|].
+        - apply/size_le0/mem_eq0 => x; rewrite mem_to_seq; [by apply/is_finite_pred|].
+          by rewrite /eq_order; apply/gtr_eqF/gt0_order.
+        move: (size_ge0 (to_seq (eq_order d))).
+        case /ler_eqVlt => [/eq_sym/size_eq0 ->/=|]; [by apply/phi_ge0|].
+        rewrite -has_predT hasP => -[x] [mem_ _]; move: (sum_phi _ lt0d) => eq_d.
+        move: (forall_ _ _ dvdd_); [by apply/ltzW|].
+        move: mem_; rewrite mem_to_seq; [by apply/is_finite_pred|].
+        move => eq_order_x; move: (size_orbit_list x); rewrite eq_order_x.
+        move => eq_size_d; rewrite -{2}eq_size_d uniq_leq_size_perm_eq.
+        - by apply/uniq_orbit_list.
+        - by apply/uniq_to_seq.
+        - move => ?; rewrite -orbit_listP ?gt0_order // => -[n] ->>.
+          rewrite mem_to_seq /=; [by apply/is_finite_pred|].
+          by rewrite -mulrM mulrC mulrM -eq_order_x intmul_order mul0i.
+        move => eq_; move/perm_eq_size: eq_ (eq_); rewrite size_orbit_list eq_sym.
+        move => eq_; move: eq_ (gt0_order x) => <-; rewrite ltrNge size_le0.
+        pose P y := _ y _ = _; move => neq_; move: (to_seq_infinite P).
+        move: neq_ => -> /=; rewrite /P => {P} is_finite_.
+        move/(perm_eq_filter (eq_order d))/perm_eq_sym => eq_.
+        move: (perm_eq_trans _ (to_seq (eq_order d)) _ _ eq_).
+        - apply/uniq_perm_eq.
+          * by apply/uniq_to_seq.
+          * by apply/filter_uniq/uniq_to_seq.
+          move => y; rewrite mem_to_seq ?is_finite_pred // mem_filter.
+          rewrite -{1}(andbT (eq_order _ _)); apply/andb_id2l.
+          rewrite eq_sym eqT => eq_order_y; rewrite mem_to_seq //=.
+          by rewrite -eq_order_y; apply/intmul_order.
+        move/perm_eq_size => ->; apply/lerr_eq; rewrite /phi.
+        rewrite -(size_map (intmul x)); apply/perm_eq_size/uniq_perm_eq.
+        - by apply/filter_uniq/uniq_orbit_list.
+        - rewrite map_inj_in_uniq; [|by apply/coprimes_uniq].
+          move => y z /coprimesP [copdy memy] /coprimesP [copdz memz].
+          move/dvd2_order; rewrite -(IntID.subr_add2r (-1)) => /eq_mod.
+          rewrite !modz_small ?gtr0_norm ?gt0_order //
+            ?eq_order_x -?mem_range ?mem_range_subr //.
+          by apply/IntID.addIr.
+        move => y; rewrite mem_filter !mapP /=; split => [[eq_order_z] [z] [+ ->>]|].
+        - rewrite range_iota /= => mem_; exists ((z - 1) %% d + 1); rewrite -eq_order_x.
+          rewrite mulrSz intmul_modz_order -mulrSz /=; apply/coprimesP.
+          rewrite mem_range_addr /=; split; last first.
+          * by rewrite -{1}(gtr0_norm _ (gt0_order x)); apply/mem_range_mod/gtr_eqF/gt0_order.
+          case/ltzE/ler_eqVlt: (gt0_order x) => [<-|gt1_orderx]; [by apply/coprime1z|].
+          rewrite modz_small /=.
+          * apply/mem_range; rewrite gtr0_norm ?gt0_order //; apply/mem_range_subr => /=.
+            move: mem_; rewrite range_ltn ?gt0_order //=; case => [->>|]; last first.
+            + by apply/mem_range_incl => //; apply/ltzW/ltzS.
+            move: eq_order_z eq_order_x; rewrite mulr0z /eq_order order0 => <<-.
+            by rewrite gtr_eqF.
+          move: eq_order_z; rewrite /eq_order order_intmul ?gt0_order // -eq_order_x.
+          rewrite -eqz_mul ?gcd_eq0 //=.
+          * by apply/negb_and; rewrite gtr_eqF //; apply/gt0_order.
+          rewrite eq_sym -subr_eq0 -mulN1r mulrC -mulrDl mulf_eq0 subr_eq0.
+          by rewrite (gtr_eqF _ _ (gt0_order x)) /coprime.
+        move => [z] [/coprimesP [coprimedz memz] ->>]; split.
+        - by rewrite /eq_order order_intmul_coprime ?gt0_order // eq_order_x.
+        exists (z %% d); rewrite range_iota /= -eq_order_x -{1}(gtr0_norm _ (gt0_order x)).
+        by rewrite mem_range_mod ?gtr_eqF ?gt0_order //= intmul_modz_order.
+      move => {forall_} forall_; move: (sum_phi _ card_gt0).
+      move: (perm_eq_flatten_filter (fun d x => eq_order d x) enum (divisors card) _).
+      + move => x _; rewrite count_filter; apply/count_eq1_eq; rewrite /predI.
+        exists (order x) => /=; do!split.
+        - apply/mem_range; rewrite -ltzS -ltr_subl_addr gt0_order /= ltzS.
+          rewrite -(gtr0_norm (order _)) ?gt0_order // -(gtr0_norm card) ?card_gt0 //.
+          by apply/dvdz_le; [apply/gtr_eqF/card_gt0|apply/dvd_order_card].
+        - by apply/dvd_order_card.
+        move => y; rewrite rem_filter ?range_uniq //.
+        by rewrite mem_filter /predC1 /eq_order eq_sym; case => ->.
+      move/perm_eq_size; rewrite {3}/card => ->; rewrite size_flatten sumzE.
+      rewrite !BIA.big_mapT; move/lerr_eq => le_; move: (ler_ge_sum_eq_seq _ _ _ _ _ le_).
+      + move => d /divisorsP [dvdd_ memd] _; rewrite /(\o) /=; move: (forall_ _ _ dvdd_).
+        - by move:memd; apply/mem_range_le.
+        apply/ler_trans/lerr_eq/perm_eq_size/uniq_perm_eq.
+        - by apply/filter_uniq/enum_uniq.
+        - by apply/uniq_to_seq.
+        move => x; rewrite mem_filter /= mem_to_seq; [by apply/is_finite_pred|].
+        by rewrite enumP.
+      move => /(_ card _ _).
+      + by apply/divisors_id/card_gt0.
+      + by rewrite /predT.
+      rewrite /(\o) /= => eq_; move: (phi_gt0 card _).
+      + by apply/ltzS/ltr_subl_addr/card_gt0.
+      move: eq_ => <- /has_predT; rewrite has_filter predTI => /hasP [g] [_] /= eq_.
+      by exists g; apply/isgeneratorP; move: eq_; rewrite /eq_order.
+    qed.
+  end FZMod.
 end FiniteZModule.
 
 (* -------------------------------------------------------------------- *)
 abstract theory FiniteComRing.
-  type t.
-
-  clone import ComRing as CR with
-    type t <= t.
+  clone include ComRingStruct.
 
   clone include FiniteZModule with
-    type t      <- t,
-    theory ZMod <= CR.
+    type t         <- t,
+    theory RL      <- RL,
+    theory ZModStr <- ZModStr
+    rename [theory] "RL"  as "Gone"
+                    "Str" as "Gone".
 
-  lemma card_gt1: 1 < FinType.card.
-  proof.
-    rewrite /FinType.card ltzE /=; have <-: size [CR.zeror; CR.oner] = 2 by trivial.
-    apply/uniq_leq_size => //=; [by rewrite eq_sym; apply/CR.oner_neq0|].
-    by move => ? _; apply/FinType.enumP.
-  qed.
+  theory FCR.
+    import FT RL ZModStr CRStr FZMod.
+
+    lemma card_gt1: 1 < FT.card.
+    proof.
+      rewrite /card ltzE /=; have <-: size [RL.zeror; RL.oner] = 2 by trivial.
+      apply/uniq_leq_size => //=; [by rewrite eq_sym; apply/RL.oner_neq0|].
+      by move => ? _; apply/enumP.
+    qed.
+
+    lemma gt0_char :
+      0 < char.
+    proof. by rewrite /char; apply/gt0_order. qed.
+
+    lemma gt1_char :
+      1 < char.
+    proof. by move/ltzE/ler_eqVlt: gt0_char; rewrite eq_sym /= neq1_char. qed.
+  end FCR.
 end FiniteComRing.
 
 (* -------------------------------------------------------------------- *)
 abstract theory FiniteIDomain.
-  type t.
-
-  clone import IDomain as ID with
-    type t <= t.
+  clone include IDomainStruct.
 
   clone include FiniteComRing with
-    type t    <- t,
-    theory ZMod <= ID,
-    theory CR <= ID.
+    type t         <- t,
+    theory RL      <- RL,
+    theory ZModStr <- ZModStr,
+    theory CRStr   <- CRStr
+    rename [theory] "RL"  as "Gone"
+                    "Str" as "Gone".
+
+  theory FID.
+    import FT RL ZModStr CRStr IDStr FZMod FCR.
+
+    lemma prime_char :
+      prime char.
+    proof. by case: char_integral => // eq0; move: gt0_char; rewrite eq0. qed.
+  
+    lemma frobenius_surj :
+      surjective frobenius.
+    proof.
+      move: (frobenius_inj prime_char) => inj_ x.
+      move: (uniq_map_injective _ _ inj_ enum_uniq) => uniq_.
+      move: (uniq_leq_size_perm_eq _ _ uniq_ enum_uniq _).
+      + by move => ? _; apply/enumP.
+      rewrite size_map /= => /perm_eq_mem /(_ x); rewrite enumP /=.
+      by move => /mapP [y] [_ ->>]; exists y.
+    qed.
+  
+    lemma frobenius_bij :
+      bijective frobenius.
+    proof.
+      by apply/bij_inj_surj; split; [apply/frobenius_inj/prime_char|apply/frobenius_surj].
+    qed.
+  
+    lemma frobenius_cr_auto :
+      cr_auto frobenius.
+    proof.
+      by split; [apply/frobenius_surj|apply/frobenius_cr_mono_endo/prime_char].
+    qed.
+  
+    lemma cr_auto_iter_frobenius n :
+      cr_auto (iter n frobenius).
+    proof. by apply/cr_auto_iter/frobenius_cr_auto. qed.
+  end FID.
 end FiniteIDomain.
 
 (* -------------------------------------------------------------------- *)
 abstract theory FiniteField.
-  type t.
-
-  clone import Field as F with
-    type t <= t.
+  clone include FieldStruct.
 
   clone include FiniteIDomain with
-    type t    <- t,
-    theory ZMod <= F,
-    theory CR <= F,
-    theory ID <= F.
-end FiniteField.
-
-
-(* ==================================================================== *)
-abstract theory FiniteZModuleStruct.
-  type t.
-
-  clone import ZModule as ZMod with
-    type t <= t.
-
-  clone import ZModuleStruct as ZModStr with
-    type t      <= t,
-    theory ZMod <= ZMod.
-
-  clone import FiniteZModule as FZMod with
-    type t      <= t,
-    theory ZMod <= ZMod.
-
-  lemma gt0_order x :
-    0 < order x.
-  proof.
-    case/ler_eqVlt: (ge0_order x) => // /eq_sym /order0P => inj_intmul.
-    by have //: false; move: inj_intmul => /=; apply/FinType.not_injective_int.
-  qed.
-
-  import StdBigop.Bigint.
-
-  lemma dvd_order_card x :
-    order x %| FinType.card.
-  proof.
-    have /(_ FinType.enum):
-      forall s , exists c ,
-        uniq c /\
-        (forall y z , y \in c => z \in c => eqv_orbit x y z => y = z) /\
-        (mem s <= mem (flatten (map (fun y => map (ZMod.(+) y) (orbit_list x)) c))).
-    + elim => [|y s [c] IHs]; [by exists [] => /=; rewrite flatten_nil|].
-      move: IHs; pose l:= flatten _; case (y \in l) => [mem_y|Nmem_y]; move => [uniq_ [forall_ mem_incl]].
-      - by exists c; split => //; split => // z /= [->>|]; [apply/mem_y|apply/mem_incl].
-      exists (y :: c); do!split => // [|z t|z] /=; [|move => [->>|mem_z] [->>|mem_t] //|].
-      - move: Nmem_y; apply/contra; rewrite /l => {l mem_incl} mem_y; apply/flatten_mapP.
-        exists y; split => //=; apply/mapP; exists zeror; rewrite /ZMod.(+) addr0 /=.
-        by apply/orbit_listP; rewrite ?gt0_order // orbit0.
-      - rewrite /eqv_orbit orbit_listP ?gt0_order //; move: Nmem_y; rewrite /l -flatten_mapP.
-        rewrite negb_exists => /= /(_ t); rewrite mem_t /= mapP negb_exists /= => /(_ (y - t)).
-        by rewrite /ZMod.(+) /ZMod.([-]) addrA addrAC subrr /= add0r.
-      - rewrite eqv_orbit_sym /eqv_orbit orbit_listP ?gt0_order //; move: Nmem_y; rewrite /l -flatten_mapP.
-        rewrite negb_exists => /= /(_ z); rewrite mem_z /= mapP negb_exists /= => /(_ (y - z)).
-        by rewrite /ZMod.(+) /ZMod.([-]) addrA addrAC subrr /= add0r.
-      - by apply/forall_.
-      rewrite flatten_cons -/l mem_cat; case => [->>|?]; [left|by right; apply/mem_incl].
-      apply/mapP; exists zeror; rewrite /ZMod.(+) addr0 /=.
-      by apply/orbit_listP; rewrite ?gt0_order // orbit0.
-    case => c; pose l:= flatten _; move => [uniq_ [forall_ mem_incl]].
-    rewrite /card (perm_eq_size _ l).
-    + apply/uniq_perm_eq; [by apply/FinType.enum_uniq| |by move => ?; split; [apply/mem_incl|move => _; apply/FinType.enumP]].
-      rewrite /l => {mem_incl l}; apply/uniq_flatten_map => //.
-      - by move => y /=; rewrite map_inj_in_uniq; [move => ? ? _ _; apply/addrI|apply/uniq_orbit_list].
-      move => y z mem_y mem_z /= /hasP [?] [] /mapP [t] [mem_t ->>] /mapP [u] [mem_u].
-      rewrite /ZMod.(+) => eq_.
-      apply/forall_ => //; move: eq_; rewrite /eqv_orbit addrC -eqr_sub => <-.
-      by apply/orbitB; apply/orbit_listP => //; apply/gt0_order.
-    rewrite /l size_flatten sumzE (BIA.eq_big_seq _ (fun _ => order x)) /=.
-    + by move => ? /mapP [?] [+ ->>]; move => /mapP [?] /= [_ ->>]; rewrite size_map size_orbit_list.
-    by rewrite BIA.sumr_const count_predT !size_map intmulz; apply/dvdz_mulr/dvdzz.
-  qed.
-
-  lemma isgeneratorP g :
-    is_generator g <=> order g = FinType.card.
-  proof.
-    rewrite /is_generator -size_orbit_list; split => [orbit_|]. search _ size perm_eq.
-    + apply/perm_eq_size/uniq_perm_eq; [by apply/uniq_orbit_list|by apply/FinType.enum_uniq|].
-      by move => x; rewrite -orbit_listP ?gt0_order // orbit_ FinType.enumP.
-    move => eq_ x; move: (uniq_leq_size_perm_eq (orbit_list g) FinType.enum).
-    rewrite orbit_listP ?gt0_order // uniq_orbit_list FinType.enum_uniq eq_ /FinType.card /= => /(_ _).
-    + by move => ? _; apply/FinType.enumP.
-    by move/perm_eq_mem => ->; apply/FinType.enumP.
-  qed.
-
-  op eq_order d x = order x = d.
-
-  lemma few_small_order_exists_generator :
-    (forall d , 0 <= d => d %| FinType.card =>
-      size (to_seq (fun x => ZMod.intmul x d = zeror)) <= d) =>
-    exists g , is_generator g.
-  proof.
-    move => forall_.
-    have: forall d , 0 <= d => d %| FinType.card => size (to_seq (eq_order d)) <= phi (d).
-    + move => d /ler_eqVlt [<<- _|lt0d dvdd_]; [rewrite phi_eq0 //|].
-      - apply/size_le0/mem_eq0 => x; rewrite mem_to_seq; [by apply/FinType.is_finite_pred|].
-        by rewrite /eq_order; apply/gtr_eqF/gt0_order.
-      move: (size_ge0 (to_seq (eq_order d))).
-      case /ler_eqVlt => [/eq_sym/size_eq0 ->/=|]; [by apply/phi_ge0|].
-      rewrite -has_predT hasP => -[x] [mem_ _]; move: (sum_phi _ lt0d) => eq_d.
-      move: (forall_ _ _ dvdd_); [by apply/ltzW|].
-      move: mem_; rewrite mem_to_seq; [by apply/FinType.is_finite_pred|].
-      move => eq_order_x; move: (size_orbit_list x); rewrite eq_order_x.
-      move => eq_size_d; rewrite -{2}eq_size_d uniq_leq_size_perm_eq.
-      - by apply/uniq_orbit_list.
-      - by apply/uniq_to_seq.
-      - move => ?; rewrite -orbit_listP ?gt0_order // => -[n] ->>.
-        rewrite mem_to_seq /=; [by apply/FinType.is_finite_pred|].
-        by rewrite /ZMod.intmul -mulrM mulrC mulrM -eq_order_x intmul_order mul0i.
-      move => eq_; move/perm_eq_size: eq_ (eq_); rewrite size_orbit_list eq_sym.
-      move => eq_; move: eq_ (gt0_order x) => <-; rewrite ltrNge size_le0.
-      pose P y := _ y _ = _; move => neq_; move: (to_seq_infinite P).
-      move: neq_ => -> /=; rewrite /P => {P} is_finite_.
-      move/(perm_eq_filter (eq_order d))/perm_eq_sym => eq_.
-      move: (perm_eq_trans _ (to_seq (eq_order d)) _ _ eq_).
-      - apply/uniq_perm_eq.
-        * by apply/uniq_to_seq.
-        * by apply/filter_uniq/uniq_to_seq.
-        move => y; rewrite mem_to_seq ?FinType.is_finite_pred // mem_filter.
-        rewrite -{1}(andbT (eq_order _ _)); apply/andb_id2l.
-        rewrite eq_sym eqT => eq_order_y; rewrite mem_to_seq //=.
-        by rewrite -eq_order_y; apply/intmul_order.
-      move/perm_eq_size => ->; apply/lerr_eq; rewrite /phi.
-      rewrite -(size_map (intmul x)); apply/perm_eq_size/uniq_perm_eq.
-      - by apply/filter_uniq/uniq_orbit_list.
-      - rewrite map_inj_in_uniq; [|by apply/coprimes_uniq].
-        move => y z /coprimesP [copdy memy] /coprimesP [copdz memz].
-        move/dvd2_order; rewrite -(IntID.subr_add2r (-1)) => /eq_mod.
-        rewrite !modz_small ?gtr0_norm ?gt0_order // ?eq_order_x -?mem_range ?mem_range_subr //.
-        by apply/IntID.addIr.
-      move => y; rewrite mem_filter !mapP /=; split => [[eq_order_z] [z] [+ ->>]|].
-      - rewrite range_iota /= => mem_; exists ((z - 1) %% d + 1); rewrite -eq_order_x.
-        rewrite mulrSz intmul_modz_order -mulrSz /=; apply/coprimesP; rewrite mem_range_addr /=.
-        split; [|by rewrite -{1}(gtr0_norm _ (gt0_order x)); apply/mem_range_mod/gtr_eqF/gt0_order].
-        case/ltzE/ler_eqVlt: (gt0_order x) => [<-|gt1_orderx]; [by apply/coprime1z|].
-        rewrite modz_small /=.
-        * apply/mem_range; rewrite gtr0_norm ?gt0_order //; apply/mem_range_subr => /=.
-          move: mem_; rewrite range_ltn ?gt0_order //=; case => [->>|]; last first.
-          + by apply/mem_range_incl => //; apply/ltzW/ltzS.
-          move: eq_order_z eq_order_x; rewrite mulr0z /eq_order order0 => <<-.
-          by rewrite gtr_eqF.
-        move: eq_order_z; rewrite /eq_order order_intmul ?gt0_order // -eq_order_x.
-        rewrite -eqz_mul ?gcd_eq0 //=; [by apply/negb_and; rewrite gtr_eqF //; apply/gt0_order|].
-        rewrite eq_sym -subr_eq0 -mulN1r mulrC -mulrDl mulf_eq0 subr_eq0.
-        by rewrite (gtr_eqF _ _ (gt0_order x)) /coprime.
-      move => [z] [/coprimesP [coprimedz memz] ->>]; split.
-      - by rewrite /eq_order order_intmul_coprime ?gt0_order // eq_order_x.
-      exists (z %% d); rewrite range_iota /= -eq_order_x -{1}(gtr0_norm _ (gt0_order x)).
-      by rewrite mem_range_mod ?gtr_eqF ?gt0_order //= intmul_modz_order.
-    move => {forall_} forall_; move: (sum_phi _ FinType.card_gt0).
-    move: (perm_eq_flatten_filter (fun d x => eq_order d x) FinType.enum (divisors FinType.card) _).
-    + move => x _; rewrite count_filter; apply/count_eq1_eq; rewrite /predI.
-      exists (order x) => /=; do!split.
-      - apply/mem_range; rewrite -ltzS -ltr_subl_addr gt0_order /= ltzS.
-        rewrite -(gtr0_norm (order _)) ?gt0_order // -(gtr0_norm FinType.card) ?FinType.card_gt0 //.
-        by apply/dvdz_le; [apply/gtr_eqF/FinType.card_gt0|apply/dvd_order_card].
-      - by apply/dvd_order_card.
-      by move => y; rewrite rem_filter ?range_uniq // mem_filter /predC1 /eq_order eq_sym; case => ->.
-    move/perm_eq_size; rewrite {3}/FinType.card => ->; rewrite size_flatten sumzE.
-    rewrite !BIA.big_mapT; move/lerr_eq => le_; move: (ler_ge_sum_eq_seq _ _ _ _ _ le_).
-    + move => d /divisorsP [dvdd_ memd] _; rewrite /(\o) /=; move: (forall_ _ _ dvdd_).
-      - by move:memd; apply/mem_range_le.
-      apply/ler_trans/lerr_eq/perm_eq_size/uniq_perm_eq.
-      - by apply/filter_uniq/FinType.enum_uniq.
-      - by apply/uniq_to_seq.
-      move => x; rewrite mem_filter /= mem_to_seq; [by apply/FinType.is_finite_pred|].
-      by rewrite FinType.enumP.
-    move => /(_ FinType.card _ _).
-    + by apply/divisors_id/FinType.card_gt0.
-    + by rewrite /predT.
-    rewrite /(\o) /= => eq_; move: (phi_gt0 FinType.card _).
-    + by apply/ltzS/ltr_subl_addr/FinType.card_gt0.
-    move: eq_ => <- /has_predT; rewrite has_filter predTI => /hasP [g] [_] /= eq_.
-    by exists g; apply/isgeneratorP; move: eq_; rewrite /eq_order.
-  qed.
-end FiniteZModuleStruct.
-
-(* -------------------------------------------------------------------- *)
-abstract theory FiniteComRingStruct.
-  type t.
-
-  clone import ComRing as CR with
-    type t <= t.
-
-  clone import ComRingStruct as CRStr with
-    type t    <= t,
-    theory CR <= CR.
-
-  clone import FiniteComRing as FCR with
-    type t    <= t,
-    theory CR <= CR.
-
-  clone include FiniteZModuleStruct with
     type t         <- t,
-    theory ZMod    <= CR,
-    theory ZModStr <= CRStr,
-    theory FZMod   <= FCR.
+    theory RL      <- RL,
+    theory ZModStr <- ZModStr,
+    theory CRStr   <- CRStr,
+    theory IDStr   <- IDStr
+    rename [theory] "RL"      as "Gone"
+                    "ZModStr" as "Gone"
+                    "CRStr"   as "Gone"
+                    "IDStr"   as "FiniteFieldFiniteIDomainIDStrGone"
+                    "FStr"    as "FiniteFieldFiniteIDomainFStrGone".
 
-  lemma gt0_char :
-    0 < char.
-  proof. by rewrite /char; apply/gt0_order. qed.
+  clone include UZMod_Field with
+    type t         <- t,
+    theory RL      <- RL,
+    theory ZModStr <- ZModStr,
+    theory CRStr   <- CRStr,
+    theory IDStr   <- IDStr,
+    theory FStr    <- FStr
+    rename [theory] "RL"      as "Gone"
+                    "ZModStr" as "Gone"
+                    "CRStr"   as "Gone"
+                    "IDStr"   as "FiniteFieldUZMod_FieldIDStrGone"
+                    "FStr"    as "FiniteFieldUZMod_FieldFStrGone".
 
-  lemma gt1_char :
-    1 < char.
-  proof. by move/ltzE/ler_eqVlt: gt0_char; rewrite eq_sym /= neq1_char. qed.
-end FiniteComRingStruct.
+  clone include FiniteZModule with
+    type t         <- uz,
+    theory RL      <- UZ,
+    theory ZModStr <- UStr
+    rename [theory] "RL"      as "Gone"
+                    "ZModStr" as "Gone"
+                    "FT"      as "FUT"
+                    "FZMod"   as "FUZMod".
 
-(* -------------------------------------------------------------------- *)
-abstract theory FiniteIDomainStruct.
-  type t.
-
-  clone import IDomain as ID with
-    type t <= t.
-
-  clone import IDomainStruct as IDStr with
-    type t    <= t,
-    theory ID <= ID.
-
-  clone import FiniteIDomain as FID with
-    type t    <= t,
-    theory ID <= ID.
-
-  clone include FiniteComRingStruct with
-    type t       <- t,
-    theory ZMod  <= ID,
-    theory CR    <= ID,
-    theory ZModStr <= IDStr,
-    theory CRStr <= IDStr,
-    theory FZMod <= FID,
-    theory FCR   <= FID.
-
-  lemma prime_char :
-    prime char.
-  proof. by case: char_integral => // eq0; move: gt0_char; rewrite eq0. qed.
-
-  lemma frobenius_bij :
-    bijective frobenius.
-  proof.
-    move: (frobenius_inj prime_char) => inj_; apply/bij_inj_surj.
-    rewrite inj_ /= => x; move: (uniq_map_injective _ _ inj_ FID.FinType.enum_uniq) => uniq_.
-    move: (uniq_leq_size_perm_eq _ _ uniq_ FID.FinType.enum_uniq _).
-    + by move => ? _; apply/FID.FinType.enumP.
-    rewrite size_map /= => /perm_eq_mem /(_ x); rewrite FID.FinType.enumP /=.
-    by move => /mapP [y] [_ ->>]; exists y.
-  qed.
-
-  lemma is_comring_automorph_frobenius :
-    is_comring_automorph frobenius.
-  proof.
-    do!split; [by apply/frobenius_bij|by apply/frobenius0/prime_char| |by apply/frobenius1|].
-    + by move => ??; apply/frobeniusD/prime_char.
-    by move => ??; apply/frobeniusM.
-  qed.
-
-  lemma is_comring_automorph_iter_frobenius n :
-    is_comring_automorph (iter n frobenius).
-  proof.
-    case (n <= 0) => [len0|/ltrNge/ltzW]; [split; split|].
-    + by exists idfun; split => ?; rewrite /idfun /= iter0.
-    + by rewrite iter0 //= => x y; rewrite !iter0.
-    + by rewrite iter0.
-    + by move => x y; rewrite !iter0.
-    elim n => [|n le0n IHn]; [split; split|].
-    + by exists idfun; split => ?; rewrite /idfun /= iter0.
-    + by rewrite iter0 //= => x y; rewrite !iter0.
-    + by rewrite iter0.
-    + by move => x y; rewrite !iter0.
-    move: (comring_automorphism_comp _ _ is_comring_automorph_frobenius IHn).
-    move: (fun_ext (iter (n + 1) frobenius) (frobenius \o iter n frobenius)).
-    by move => [_ ->] // x; rewrite iterS.
-  qed.
-end FiniteIDomainStruct.
-
-(* -------------------------------------------------------------------- *)
-abstract theory FiniteFieldStruct.
-  type t, ut.
-
-  clone import Field as F with
-    type t <= t.
-
-  clone import FieldStruct as FStr with
-    type t   <= t,
-    theory F <= F.
-
-  clone import FiniteField as FF with
-    type t   <= t,
-    theory F <= F.
-
-  clone include FiniteIDomainStruct with
-    type t       <- t,
-    theory ZMod  <= F,
-    theory CR    <= F,
-    theory ID    <= F,
-    theory ZModStr <= FStr,
-    theory CRStr <= FStr,
-    theory IDStr <= FStr,
-    theory FZMod <= FF,
-    theory FCR   <= FF,
-    theory FID   <= FF.
-
-  clone import UZMod_Field as UF with
-    type t   <= t,
-    type uz  <= ut,
-    theory F <= F.
-
-  (*TODO: this could be done in FiniteIDomainStruct, if only unit was an op and not a pred.*)
-  clone import SubFinite as SFU with
-    type t    <= t,
-    type st   <= ut,
-    op p      <= (fun x => x <> zeror),
-    theory FT <= FF.FinType.
-
-  (*TODO: two equivalent FinType.*)
-  print SFU.Sub.
-  print UF.Sub.
-
-  clone import FiniteZModuleStruct as UFStr with
-    type t <= ut,
-    theory ZMod <= UF.UZMod,
-    theory FZMod.FinType <= SFU.SFT.
-
-  lemma card_unit :
-    FF.FinType.card = SFU.SFT.card + 1.
-  proof.
-    rewrite /card (perm_eq_size  _ _ (perm_to_rem _ _ (FinType.enumP zeror))) /=.
-    rewrite addrC; congr; rewrite -(size_map Sub.val); apply/perm_eq_size/uniq_perm_eq.
-    + by apply/rem_uniq/FinType.enum_uniq.
-    + by apply/uniq_map_injective; [apply/Sub.val_inj|apply/SFT.enum_uniq].
-    move => x; case: (x = zeror) => [->>|neqx0].
-    + rewrite /senum -map_comp; pose s:= filter _ _.
-      case: (eq_in_map (Sub.val \o Sub.insubd) idfun s).
-      rewrite /s => + _ {s}; move => -> /=.
-      + by move => x /mem_filter /= [neqx0 _]; rewrite /(\o) /idfun /= Sub.val_insubd neqx0.
-      by rewrite map_id mem_filter /= rem_filter ?FinType.enum_uniq // mem_filter /predC1.
-    rewrite mem_rem_neq // 1?eq_sym // FinType.enumP /=; apply/mapP.
-    by exists (Sub.insubd x); rewrite SFT.enumP /= Sub.val_insubd neqx0.
-  qed.
-
-  lemma exists_generator :
-    exists (g : ut), UFStr.ZModStr.is_generator g.
-  proof.
-    apply/few_small_order_exists_generator => d.
-    case/ler_eqVlt => [<<- /dvd0z|lt0d]; [by move => eq_; move: SFT.card_gt0; rewrite eq_|].
-    move => dvdd_; move: (size_to_seq_eq_pow_1 _ lt0d); apply/ler_trans/lerr_eq.
-    rewrite -(size_map UF.Sub.insubd); apply/perm_eq_size/uniq_perm_eq.
-    + by apply/uniq_to_seq.
-    + rewrite map_inj_in_uniq; [|by apply/uniq_to_seq].
-      move => x y; rewrite !mem_to_seq ?FinType.is_finite_pred //.
-      move => eqx eqy /(congr1 UF.Sub.val); rewrite !UF.Sub.insubdK //.
-      - by apply/(unitrX_neq0 _ d); [apply/gtr_eqF|rewrite eqx unitr1].
-      by apply/(unitrX_neq0 _ d); [apply/gtr_eqF|rewrite eqy unitr1].
-    move => x; rewrite mapP mem_to_seq ?SFT.is_finite_pred //=.
-    rewrite /eq_pow_1; split => [eq_|[y] [+ ->>]].
-    + exists (UF.Sub.val x); rewrite UF.Sub.valKd /= mem_to_seq ?FinType.is_finite_pred //=.
-      by rewrite -UF.val_intmul; move: eq_; rewrite /FZMod.ZMod.intmul => ->; rewrite val1.
-    rewrite mem_to_seq ?FinType.is_finite_pred //= => eq_.
-    apply/UF.Sub.val_inj; rewrite UF.val_intmul val1 UF.Sub.insubdK //.
-    by apply/(unitrX_neq0 _ d); [apply/gtr_eqF|rewrite eq_ unitr1].
-  qed.
-end FiniteFieldStruct.
-
+  theory FF.
+    import FT RL ZModStr CRStr IDStr FStr FZMod FCR FID.
+    import UZ UStr USub FUT FUZMod.
+  
+    lemma card_unit :
+      FT.card = FUT.card + 1.
+    proof.
+      rewrite /card (perm_eq_size  _ _ (perm_to_rem _ _ (FT.enumP RL.zeror))) /=.
+      rewrite addrC; congr; rewrite -(size_map USub.val); apply/perm_eq_size/uniq_perm_eq.
+      + by apply/rem_uniq/FT.enum_uniq.
+      + by apply/uniq_map_injective; [apply/USub.val_inj|apply/FUT.enum_uniq].
+      move => x; case: (x = RL.zeror) => [->>|neqx0].
+      + rewrite rem_filter ?FT.enum_uniq // mem_filter /predC1 /= mapP.
+        rewrite negb_exists /= => u; rewrite FUT.enumP /= eq_sym.
+        by apply/negP; move/(congr1 unit); rewrite valP unitr0.
+      rewrite mem_rem_neq // 1?eq_sym // FT.enumP /=; apply/mapP.
+      by exists (insubd x); rewrite FUT.enumP /= val_insubd unitfP.
+    qed.
+  
+    lemma exists_generator :
+      exists g, UStr.is_generator g.
+    proof.
+      apply/few_small_order_exists_generator => d.
+      case/ler_eqVlt => [<<- /dvd0z|lt0d]; [by move => eq_; move: FUT.card_gt0; rewrite eq_|].
+      move => dvdd_; move: (size_to_seq_eq_pow_1 _ lt0d); apply/ler_trans/lerr_eq.
+      rewrite -(size_map USub.insubd); apply/perm_eq_size/uniq_perm_eq.
+      + by apply/uniq_to_seq.
+      + rewrite map_inj_in_uniq; [|by apply/uniq_to_seq].
+        move => x y; rewrite !mem_to_seq ?FT.is_finite_pred //.
+        move => eqx eqy /(congr1 USub.val); rewrite !USub.insubdK //.
+        - by apply/(unitrX_neq0 _ d); [apply/gtr_eqF|rewrite eqx unitr1].
+        by apply/(unitrX_neq0 _ d); [apply/gtr_eqF|rewrite eqy unitr1].
+      move => x; rewrite mapP mem_to_seq ?FUT.is_finite_pred //=.
+      rewrite /eq_pow_1; split => [eq_|[y] [+ ->>]].
+      + exists (USub.val x); rewrite USub.valKd /= mem_to_seq ?FT.is_finite_pred //=.
+        by rewrite -UZModCR.valX eq_ val_insubd unitr1.
+      rewrite mem_to_seq ?FT.is_finite_pred //= => eq_.
+      apply/USub.val_inj; rewrite UZModCR.valX UZModCR.val1 USub.insubdK //.
+      by apply/(unitrX_neq0 _ d); [apply/gtr_eqF|rewrite eq_ unitr1].
+    qed.
+  end FF.
+end FiniteField.
 
 (* ==================================================================== *)
 abstract theory SubFiniteZModule.
-  type t, st.
+  type t.
 
-  clone import ZModule as ZMod with
-    type t <= t.
+  op P : t -> bool.
 
-  clone import SubZModule as SubZMod with
-    type t      <= t,
-    type st     <= st,
-    theory ZMod <- ZMod.
-
-  clone import FiniteZModule as FZMod with
-    type t      <= t,
-    theory ZMod <= ZMod.
-
-  clone import ZModuleStruct as ZModStr with
-    type t      <= t,
-    theory ZMod <= ZMod.
-
-  clone import FiniteZModuleStruct as FZModStr with
-    type t         <= t,
-    theory ZMod    <= ZMod,
-    theory ZModStr <= ZModStr,
-    theory FZMod   <= FZMod.
+  clone include SubZModule with
+    type t <- t,
+    pred Sub.P <= P.
 
   clone include SubFinite with
     type t     <- t,
     type st    <- st,
-    op p       <- p,
-    theory FT  <= FZMod.FinType,
-    theory Sub <= SubZMod.Sub.
+    op P       <- P,
+    theory Sub <- Sub
+    rename [theory] "Sub" as "Gone".
 
-  clone import FiniteZModule as SFZMod with
-    type t                  <= st,
-    theory ZMod             <= SZMod,
-    theory FinType          <= SFT.
+  clone include FiniteZModule with
+    type t         <- t,
+    theory RL      <- TRL,
+    theory ZModStr <- ZModTStr,
+    theory FT      <- TFT
+    rename [theory] "FZMod" as "FZModT".
+
+  clone include FiniteZModule with
+    type t         <- st,
+    theory RL      <- SRL,
+    theory ZModStr <- ZModSStr,
+    theory FT      <- SFT
+    rename [theory] "FZMod" as "FZModS".
 end SubFiniteZModule.
 
 (* -------------------------------------------------------------------- *)
 abstract theory SubFiniteComRing.
-  type t, st.
+  type t.
 
-  clone import ComRing as CR with
-    type t <= t.
+  op P : t -> bool.
 
-  clone import ComRingPred as CRPr with
-    type t    <= t,
-    theory CR <= CR.
-
-  clone import SubComRing as SubCR with
-    type t      <= t,
-    type st     <= st,
-    theory CR   <= CR,
-    theory CRPr <= CRPr.
-
-  clone import FiniteComRing as FCR with
-    type t    <= t,
-    theory CR <= CR.
-
-  clone import ComRingStruct as CRStr with
-    type t    <= t,
-    theory CR <= CR.
-
-  clone import FiniteComRingStruct as FCRStr with
-    type t       <= t,
-    theory CR    <= CR,
-    theory CRStr <= CRStr,
-    theory FCR   <= FCR.
-
-  clone import SubComRingModule as SCRM with
-    type t            <= t,
-    type st           <= st,
-    theory CR         <= CR,
-    theory CRPr       <= CRPr,
-    theory SubCR      <= SubCR.
+  clone include SubComRingModule with
+    type t <- t,
+    pred Sub.P <= P.
 
   clone include SubFiniteZModule with
-    type t          <- t,
-    type st         <- st,
-    theory ZMod     <= CR,
-    theory SubZMod  <= SubCR,
-    theory FZMod    <= FCR,
-    theory ZModStr  <= CRStr,
-    theory FZModStr <= FCRStr,
-    theory FT  <= FinType,
-    theory Sub <= SubCR.Sub.
+    type t           <- t,
+    type st          <- st,
+    op P             <- P,
+    theory TRL       <- TRL,
+    theory SRL       <- SRL,
+    theory ZModTStr  <- ZModTStr,
+    theory ZModSStr  <- ZModSStr,
+    theory ZModMorph <- ZModMorph,
+    theory SZMod     <- SZMod,
+    theory Sub       <- Sub
+    rename [theory] "TRL"   as "Gone"
+                    "SRL"   as "Gone"
+                    "Str"   as "Gone"
+                    "Morph" as "Gone"
+                    "SZMod" as "Gone"
+                    "Sub"   as "Gone".
 
-  clone import FiniteComRing as SFCR with
-    type t          <= st,
-    theory CR       <= SCR,
-    theory FinType  <= SFT.
+  clone include FiniteComRing with
+    type t         <- t,
+    theory RL      <- TRL,
+    theory ZModStr <- ZModTStr,
+    theory CRStr   <- CRTStr,
+    theory FT      <- TFT,
+    theory FZMod   <- FZModT
+    rename [theory] "FZMod" as "Gone"
+                    "FCR"   as "FCRT".
 
-  import SCRM.CRM.
+  clone include FiniteComRing with
+    type t         <- st,
+    theory RL      <- SRL,
+    theory ZModStr <- ZModSStr,
+    theory CRStr   <- CRSStr,
+    theory FT      <- SFT,
+    theory FZMod   <- FZModS
+    rename [theory] "FZMod" as "Gone"
+                    "FCR"   as "FCRS".
 
-  op enum_lin (vs : t list) =
-    map
-      (fun ss => lin ss vs)
-      (foldr (allpairs (::)) [[]] (nseq (size vs) senum)).
+  theory SFCR.
+    import TRL SRL ZModTStr ZModSStr CRTStr CRSStr ZModMorph CRMorph SZMod SCR Sub CRM.
+    import TFT SFT.
 
-  lemma enum_lin_nil :
-    enum_lin [] = [SubFiniteComRing.CR.zeror].
-  proof. by rewrite /enum_lin /= nseq0 /= BigZMod.big_nil. qed.
-
-  lemma enum_lin_cons v vs :
-    enum_lin (v :: vs) =
-    allpairs SubFiniteComRing.CR.( + ) (map (transpose SCRM.( ** ) v) senum) (enum_lin vs).
-  proof.
-    rewrite /enum_lin /= addrC nseqS ?size_ge0 //=; pose el := foldr _ _ _.
-    elim: senum el => [|x senum IHsenum] el /=; [by rewrite !allpairs0l|].
-    rewrite !allpairs_consl map_cat IHsenum -!map_comp; congr => {IHsenum}.
-    by apply/eq_map => xs; rewrite /(\o) /= BigZMod.big_cons /predT /idfun.
-  qed.
-
-  lemma enum_linP vs v :
-    (v \in enum_lin vs) <=> (gen (vf_oflist vs) v).
-  proof.
-    elim: vs v => [|v vs IHvs] w.
-    + by rewrite enum_lin_nil gen_vf_oflist_nil.
-    rewrite enum_lin_cons gen_vf_oflist_cons allpairsP; split.
-    + case => -[v1 v2] /= |> /mapP [s] |> mem_s /IHvs gen_v2.
-      by exists s SCR.oner v2; rewrite gen_v2 scale1r.
-    case => [s1 s2 w2] /= |> /(gen_scale _ s2) /IHvs mem_w2.
-    exists (s1 ** v, s2 ** w2)%SCRM; rewrite mem_w2 /=.
-    by apply/mapP; exists s1 => /=; apply/SFT.enumP.
-  qed.
-
-  lemma size_enum_lin vs :
-    size (enum_lin vs) = SFT.card ^ (size vs).
-  proof.
-    elim: vs => [|v vs IHvs] /=.
-    + by rewrite expr0 enum_lin_nil.
-    rewrite addrC exprS ?size_ge0 // -IHvs => {IHvs}.
-    rewrite /enum_lin !size_map /= addrC nseqS ?size_ge0 //=.
-    by rewrite size_allpairs /SFT.card size_map.
-  qed.
-
-  lemma free_uniq_enum_lin vs :
-    uniq vs =>
-    free (vf_oflist vs) =>
-    uniq (enum_lin vs).
-  proof.
-    elim: vs => [|v vs IHvs]; [by rewrite enum_lin_nil|].
-    rewrite free_vf_oflist_cons enum_lin_cons /=.
-    move => |> Nmem_v uniq_ imp_eq0 free_.
-    rewrite allpairs_mapl; apply/allpairs_uniq.
-    + by apply/SFT.enum_uniq.
-    + by apply/IHvs.
-    move => s1 s2 v1 v2 mem_s1 mem_s2 /enum_linP gen1 /enum_linP gen2 /=.
-    rewrite addrC -eqr_sub -scaleNr -scaleDl => eq_.
-    move/(_ (s2 + (-s1))%SCR _): imp_eq0.
-    + by rewrite -eq_; apply/gen_add => //; apply/gen_opp.
-    by rewrite SCR.subr_eq0 => ->>; move: eq_; rewrite /= SCR.subrr scale0r SubFiniteComRing.CR.subr_eq0.
-  qed.
-
-  lemma gen_t_enum_lin vs :
-    (gen_t (vf_oflist vs)) <=> (forall v , v \in enum_lin vs).
-  proof. by rewrite /gen_t; apply/forall_eq => v /=; apply/eqboolP; rewrite enum_linP. qed.
+    op enum_lin (vs : t list) =
+      map
+        (fun ss => lin ss vs)
+        (foldr (allpairs (::)) [[]] (nseq (size vs) SFT.enum)).
+  
+    lemma enum_lin_nil :
+      enum_lin [] = [TRL.zeror].
+    proof. by rewrite /enum_lin /= nseq0 /= BigMod.big_nil. qed.
+  
+    lemma enum_lin_cons v vs :
+      enum_lin (v :: vs) =
+      allpairs TRL.( + ) (map (transpose CRM.( ** ) v) SFT.enum) (enum_lin vs).
+    proof.
+      rewrite /enum_lin /= addrC nseqS ?size_ge0 //=; pose el := foldr _ _ _.
+      elim: SFT.enum el => [|x senum IHsenum] el /=; [by rewrite !allpairs0l|].
+      rewrite !allpairs_consl map_cat IHsenum -!map_comp; congr => {IHsenum}.
+      by apply/eq_map => xs; rewrite /(\o) /= BigMod.big_cons /predT /idfun.
+    qed.
+  
+    lemma enum_linP vs v :
+      (v \in enum_lin vs) <=> (gen (vf_oflist vs) v).
+    proof.
+      elim: vs v => [|v vs IHvs] w.
+      + by rewrite enum_lin_nil gen_vf_oflist_nil.
+      rewrite enum_lin_cons gen_vf_oflist_cons allpairsP; split.
+      + case => -[v1 v2] /= |> /mapP [s] |> mem_s /IHvs gen_v2.
+        by exists s SRL.oner v2; rewrite gen_v2 scale1r.
+      case => [s1 s2 w2] /= |> /(gen_scale _ s2) /IHvs mem_w2.
+      exists (s1 ** v, s2 ** w2)%CRM; rewrite mem_w2 /=.
+      split; last by rewrite /CRM.( ** ).
+      by apply/mapP; exists s1 => /=; apply/SFT.enumP.
+    qed.
+  
+    lemma size_enum_lin vs :
+      size (enum_lin vs) = SFT.card ^ (size vs).
+    proof.
+      elim: vs => [|v vs IHvs] /=.
+      + by rewrite expr0 enum_lin_nil.
+      rewrite addrC exprS ?size_ge0 // -IHvs => {IHvs}.
+      rewrite /enum_lin !size_map /= addrC nseqS ?size_ge0 //=.
+      by rewrite size_allpairs -/SFT.card.
+    qed.
+  
+    lemma free_uniq_enum_lin vs :
+      uniq vs =>
+      free (vf_oflist vs) =>
+      uniq (enum_lin vs).
+    proof.
+      elim: vs => [|v vs IHvs]; [by rewrite enum_lin_nil|].
+      rewrite free_vf_oflist_cons enum_lin_cons /=.
+      move => |> Nmem_v uniq_ imp_eq0 free_.
+      rewrite allpairs_mapl; apply/allpairs_uniq.
+      + by apply/SFT.enum_uniq.
+      + by apply/IHvs.
+      move => s1 s2 v1 v2 mem_s1 mem_s2 /enum_linP gen1 /enum_linP gen2 /=.
+      rewrite addrC -eqr_sub -scaleNr -scaleDl => eq_.
+      move/(_ (s2 + (-s1))%SRL _): imp_eq0.
+      + by rewrite -eq_; apply/gen_add => //; apply/gen_opp.
+      rewrite SRL.subr_eq0 => ->>; move: eq_.
+      by rewrite /= SRL.subrr scale0r TRL.subr_eq0.
+    qed.
+  
+    lemma gen_t_enum_lin vs :
+      (gen_t (vf_oflist vs)) <=> (forall v , v \in enum_lin vs).
+    proof. by rewrite /gen_t; apply/forall_eq => v /=; apply/eqboolP; rewrite enum_linP. qed.
+  end SFCR.
 end SubFiniteComRing.
 
 (* -------------------------------------------------------------------- *)
 abstract theory SubFiniteIDomain.
-  type t, st.
+  type t.
 
-  clone import IDomain as ID with
-    type t <= t.
+  op P : t -> bool.
 
-  clone import IDomainPred as IDPr with
-    type t    <= t,
-    theory ID <= ID.
-
-  clone import SubIDomain as SubID with
-    type t      <= t,
-    type st     <= st,
-    theory ID   <= ID,
-    theory IDPr <= IDPr.
-
-  clone import FiniteIDomain as FID with
-    type t    <= t,
-    theory ID <= ID.
-
-  clone import IDomainStruct as IDStr with
-    type t    <= t,
-    theory ID <= ID.
-
-  clone import FiniteIDomainStruct as FIDStr with
-    type t       <= t,
-    theory ID    <= ID,
-    theory IDStr <= IDStr,
-    theory FID   <= FID.
-
-  clone import SubIDomainModule as SIDM with
-    type t            <= t,
-    type st           <= st,
-    theory ID         <= ID,
-    theory IDPr       <= SubFiniteIDomain.IDPr,
-    theory SubID      <= SubFiniteIDomain.SubID.
+  clone include SubIDomainModule with
+    type t <- t,
+    pred Sub.P <= P.
 
   clone include SubFiniteComRing with
-    type t            <- t,
-    type st           <- st,
-    theory ZMod       <= ID,
-    theory CR         <= ID,
-    theory CRPr       <= IDPr,
-    theory SubZMod    <= SubID,
-    theory SubCR      <= SubID,
-    theory FZMod      <= FID,
-    theory FCR        <= FID,
-    theory ZModStr    <= IDStr,
-    theory CRStr      <= IDStr,
-    theory FZModStr   <= FIDStr,
-    theory FCRStr     <= FIDStr,
-    theory FT         <= FinType,
-    theory Sub        <= SubID.Sub,
-    theory SCRM       <= SIDM.
+    type t           <- t,
+    type st          <- st,
+    op P             <- P,
+    theory TRL       <- TRL,
+    theory SRL       <- SRL,
+    theory ZModTStr  <- ZModTStr,
+    theory ZModSStr  <- ZModSStr,
+    theory CRTStr    <- CRTStr,
+    theory CRSStr    <- CRSStr,
+    theory ZModMorph <- ZModMorph,
+    theory CRMorph   <- CRMorph,
+    theory SZMod     <- SZMod,
+    theory SCR       <- SCR,
+    theory CRM       <- CRM,
+    theory Sub       <- Sub
+    rename [theory] "TRL"   as "Gone"
+                    "SRL"   as "Gone"
+                    "Str"   as "Gone"
+                    "Morph" as "Gone"
+                    "SZMod" as "Gone"
+                    "SCR"   as "Gone"
+                    "CRM"   as "Gone"
+                    "Sub"   as "Gone".
 
-  clone import FiniteIDomain as SFID with
-    type t          <= st,
-    theory ID       <= SID,
-    theory FinType  <= SFT.
+  clone include FiniteIDomain with
+    type t         <- t,
+    theory RL      <- TRL,
+    theory ZModStr <- ZModTStr,
+    theory CRStr   <- CRTStr,
+    theory IDStr   <- IDTStr,
+    theory FT      <- TFT,
+    theory FZMod   <- FZModT,
+    theory FCR     <- FCRT
+    rename [theory] "FZMod" as "Gone"
+                    "FCR"   as "Gone"
+                    "FID"   as "FIDT"
+                    "IDStr" as "FiniteIDomainTIDStrGone".
+
+  clone include FiniteIDomain with
+    type t         <- st,
+    theory RL      <- SRL,
+    theory ZModStr <- ZModSStr,
+    theory CRStr   <- CRSStr,
+    theory IDStr   <- IDSStr,
+    theory FT      <- SFT,
+    theory FZMod   <- FZModS,
+    theory FCR     <- FCRS
+    rename [theory] "FZMod" as "Gone"
+                    "FCR"   as "Gone"
+                    "FID"   as "FIDS"
+                    "IDStr" as "FiniteIDomainSIDStrGone".
 end SubFiniteIDomain.
 
 (* -------------------------------------------------------------------- *)
 abstract theory SubFiniteField.
-  type t, st, ut.
+  type t.
 
-  clone import Field as F with
-    type t <= t.
+  op P : t -> bool.
 
-  clone import FieldPred as FPr with
-    type t   <= t,
-    theory F <= F.
-
-  clone import SubField as SubF with
-    type t     <= t,
-    type st    <= st,
-    theory F   <= F,
-    theory FPr <= FPr.
-
-  clone import FiniteField as FF with
-    type t   <= t,
-    theory F <= F.
-
-  clone import FieldStruct as FStr with
-    type t   <= t,
-    theory F <= F.
-
-  clone import FiniteFieldStruct as FFStr with
-    type t      <= t,
-    type ut     <= ut,
-    theory F    <= F,
-    theory FStr <= FStr,
-    theory FF   <= FF.
-
-  clone import SubVectorSpace as SVS with
-    type t          <= t,
-    type st         <= st,
-    theory F        <= F,
-    theory FPr      <= SubFiniteField.FPr,
-    theory SubF     <= SubF.
+  clone include SubVectorSpace with
+    type t <- t,
+    pred Sub.P <= P.
 
   clone include SubFiniteIDomain with
-    type t            <- t,
-    type st           <- st,
-    theory ZMod       <= F,
-    theory CR         <= F,
-    theory ID         <= F,
-    theory CRPr       <= FPr,
-    theory IDPr       <= FPr,
-    theory SubZMod    <= SubF,
-    theory SubCR      <= SubF,
-    theory SubID      <= SubF,
-    theory FZMod      <= FF,
-    theory FCR        <= FF,
-    theory FID        <= FF,
-    theory ZModStr    <= FStr,
-    theory CRStr      <= FStr,
-    theory IDStr      <= FStr,
-    theory FZModStr   <= FFStr,
-    theory FCRStr     <= FFStr,
-    theory FIDStr     <= FFStr,
-    theory FT         <= FinType,
-    theory Sub        <= SubID.Sub,
-    theory SCRM       <= SVS,
-    theory SIDM       <= SVS.
+    type t           <- t,
+    type st          <- st,
+    op P             <- P,
+    theory TRL       <- TRL,
+    theory SRL       <- SRL,
+    theory ZModTStr  <- ZModTStr,
+    theory ZModSStr  <- ZModSStr,
+    theory CRTStr    <- CRTStr,
+    theory CRSStr    <- CRSStr,
+    theory IDTStr    <- IDTStr,
+    theory IDSStr    <- IDSStr,
+    theory ZModMorph <- ZModMorph,
+    theory CRMorph   <- CRMorph,
+    theory IDMorph   <- IDMorph,
+    theory SZMod     <- SZMod,
+    theory SCR       <- SCR,
+    theory SID       <- SID,
+    theory CRM       <- CRM,
+    theory Sub       <- Sub
+    rename [theory] "TRL"       as "Gone"
+                    "SRL"       as "Gone"
+                    "ZModTStr"  as "Gone"
+                    "ZModSStr"  as "Gone"
+                    "CRTStr"    as "Gone"
+                    "CRSStr"    as "Gone"
+                    "IDTStr"    as "SubFiniteFieldIDTStrGone"
+                    "IDSStr"    as "SubFiniteFieldIDSStrGone"
+                    "IDStr1"    as "SubFiniteFieldIDStr1Gone"
+                    "IDStr2"    as "SubFiniteFieldIDStr2Gone"
+                    "ZModMorph" as "Gone"
+                    "CRMorph"   as "Gone"
+                    "IDMorph"   as "SubFiniteFieldIDMorphGone"
+                    "SZMod"     as "Gone"
+                    "SCR"       as "Gone"
+                    "SID"       as "Gone"
+                    "CRM"       as "Gone"
+                    "Sub"       as "Gone".
 
-  clone import FiniteField as SFF with
-    type t          <= st,
-    theory F        <= SF,
-    theory FinType  <= SFT.
+  clone include FiniteField with
+    type t         <- t,
+    theory RL      <- TRL,
+    theory ZModStr <- ZModTStr,
+    theory CRStr   <- CRTStr,
+    theory IDStr   <- IDTStr,
+    theory FStr    <- FTStr,
+    theory FT      <- TFT,
+    theory FZMod   <- FZModT,
+    theory FCR     <- FCRT,
+    theory FID     <- FIDT
+    rename [theory] "FZMod" as "Gone"
+                    "FCR"   as "Gone"
+                    "FID"   as "Gone"
+                    "FF"    as "FFT"
+                    "IDStr" as "FiniteFieldTIDStrGone"
+                    "FStr"  as "FiniteFieldTFStrGone"
+                    "UZ"    as "UZT"
+                    "UStr"  as "UTStr"
+                    "UFZMod" as "UFZModT"
+                    "USub"  as "USubT"
+                    "FUT"   as "FUTT"
+           [type]   "uz"    as "uzt".
 
-  import SVS.VS.
+  clone include FiniteField with
+    type t         <- st,
+    theory RL      <- SRL,
+    theory ZModStr <- ZModSStr,
+    theory CRStr   <- CRSStr,
+    theory IDStr   <- IDSStr,
+    theory FStr    <- FSStr,
+    theory FT      <- SFT,
+    theory FZMod   <- FZModS,
+    theory FCR     <- FCRS,
+    theory FID     <- FIDS
+    rename [theory] "FZMod" as "Gone"
+                    "FCR"   as "Gone"
+                    "FID"   as "Gone"
+                    "FF"    as "FFS"
+                    "IDStr" as "FiniteFieldSIDStrGone"
+                    "FStr"  as "FiniteFieldSFStrGone"
+                    "UZ"    as "UZS"
+                    "UStr"  as "USStr"
+                    "USub"  as "USubS"
+                    "FUT"   as "FUTS"
+           [type]   "uz"    as "uzs".
 
-  lemma finite_basis_exists :
-    exists vs , uniq vs /\ basis (vf_oflist vs).
-  proof.
-    have /(_ FF.FinType.card):
-      forall n , 0 <= n => n <= FF.FinType.card =>
-      exists vs , uniq vs /\ free (vf_oflist vs) /\ n <= size (enum_lin vs);
-    last first.
-    + rewrite size_ge0 /= => -[vs] |> uniq_ free_ lecn.
-      exists vs; rewrite uniq_ /basis free_ /= gen_t_enum_lin => v.
-      move: lecn; rewrite uniq_leq_size_perm_eq.
-      - by apply/free_uniq_enum_lin.
-      - by apply/FF.FinType.enum_uniq.
-      - by move => ? _; apply/FF.FinType.enumP.
-      by move => /perm_eq_mem ->; apply/FF.FinType.enumP.
-    elim => [_|n le0n IHn /ltzE ltnc].
-    + by exists []; rewrite free_vf_oflist_nil size_ge0.
-    case/(_ _): IHn => [|vs |> uniq_ free_]; [by apply/ltzW|].
-    move => /ler_eqVlt [->>|ltnp]; [|by exists vs; rewrite -ltzE].
-    move/ltzNge: ltnc; rewrite uniq_leq_size_perm_eq.
-    + by apply/free_uniq_enum_lin.
-    + by apply/FF.FinType.enum_uniq.
-    + by move => ? _; apply/FF.FinType.enumP.
-    move => Nperm_eq_; move: (uniq_perm_eq (enum_lin vs) FF.FinType.enum _ _).
-    + by apply/free_uniq_enum_lin.
-    + by apply/FF.FinType.enum_uniq.
-    rewrite Nperm_eq_ /= negb_forall /= => -[v]; rewrite FF.FinType.enumP /= => Nmemv.
-    exists (v :: vs); rewrite /= free_vf_oflist_cons uniq_ free_ /=; do!split.
-    + by move: Nmemv; apply/contra => memv; apply/enum_linP/gen_p.
-    + right => s; case: (s = SCR.zeror) => [->> //=|neqs0].
-      rewrite -gen_scale_unit -?enum_linP //; apply/unitfP.
-      by move: neqs0; apply/contra => ?; apply/Sub.val_inj; rewrite val0.
-    rewrite !size_enum_lin /= -ltzE addrC exprSr ?size_ge0 //.
-    rewrite -subr_gt0 -IntID.mulN1r mulrC -IntID.mulrDl; apply/mulr_gt0.
-    + by rewrite subr_gt0; apply/card_gt1.
-    by apply/expr_gt0/SFT.card_gt0.
-  qed.
+  theory SFF.
+    import TRL SRL ZModTStr ZModSStr CRTStr CRSStr IDTStr IDSStr FTStr FSStr.
+    import ZModMorph CRMorph IDMorph FMorph SZMod SCR SID SF Sub CRM.
+    import TFT SFT SFCR.
 
-  op n = ilog SFT.card FF.FinType.card.
-
-  lemma lt0n :
-    0 < n.
-  proof.
-    rewrite /n ltzE /=; move: (ilog_mono SFT.card SFT.card FF.FinType.card).
-    rewrite ilog_b SFCR.card_gt1 SFT.card_gt0 /= => -> //.
-    by rewrite /SFT.card /FinType.card /senum size_map size_filter count_size.
-  qed.
-
-  lemma eq_card_pow_n :
-    FF.FinType.card = SFT.card ^ n.
-  proof.
-    case: finite_basis_exists => vs [uniq_ basis_].
-    case: (basis_) => free_ /gen_t_enum_lin mem_e.
-    move: (free_uniq_enum_lin _ uniq_ free_) => uniq_e.
-    move: (size_enum_lin vs); rewrite /n /FF.FinType.card /SubFiniteField.FF.FinType.card.
-    rewrite (perm_eq_size _ FF.FinType.enum).
-    + apply/uniq_perm_eq => // [|x]; [by apply/FF.FinType.enum_uniq|].
-      by rewrite FF.FinType.enumP mem_e.
-    by move=> ->; rewrite ilog_powK // SFCR.card_gt1.
-  qed.
+    lemma finite_basis_exists :
+      exists vs , uniq vs /\ basis (vf_oflist vs).
+    proof.
+      have /(_ TFT.card):
+        forall n , 0 <= n => n <= TFT.card =>
+        exists vs , uniq vs /\ free (vf_oflist vs) /\ n <= size (enum_lin vs);
+      last first.
+      + rewrite size_ge0 /= => -[vs] |> uniq_ free_ lecn.
+        exists vs; rewrite uniq_ /basis free_ /= gen_t_enum_lin => v.
+        move: lecn; rewrite uniq_leq_size_perm_eq.
+        - by apply/free_uniq_enum_lin.
+        - by apply/TFT.enum_uniq.
+        - by move => ? _; apply/TFT.enumP.
+        by move => /perm_eq_mem ->; apply/TFT.enumP.
+      elim => [_|n le0n IHn /ltzE ltnc].
+      + by exists []; rewrite free_vf_oflist_nil size_ge0.
+      case/(_ _): IHn => [|vs |> uniq_ free_]; [by apply/ltzW|].
+      move => /ler_eqVlt [->>|ltnp]; [|by exists vs; rewrite -ltzE].
+      move/ltzNge: ltnc; rewrite uniq_leq_size_perm_eq.
+      + by apply/free_uniq_enum_lin.
+      + by apply/TFT.enum_uniq.
+      + by move => ? _; apply/TFT.enumP.
+      move => Nperm_eq_; move: (uniq_perm_eq (enum_lin vs) TFT.enum _ _).
+      + by apply/free_uniq_enum_lin.
+      + by apply/TFT.enum_uniq.
+      rewrite Nperm_eq_ /= negb_forall /= => -[v]; rewrite TFT.enumP /= => Nmemv.
+      exists (v :: vs); rewrite /= free_vf_oflist_cons uniq_ free_ /=; do!split.
+      + by move: Nmemv; apply/contra => memv; apply/enum_linP/gen_p.
+      + right => s; case: (s = SRL.zeror) => [->> //=|neqs0].
+        rewrite -gen_scale_unit -?enum_linP //; apply/unitfP.
+        by move: neqs0; apply/contra => ->>; apply/Sub.val_inj; rewrite val0.
+      rewrite !size_enum_lin /= -ltzE addrC exprSr ?size_ge0 //.
+      rewrite -subr_gt0 -IntID.mulN1r mulrC -IntID.mulrDl; apply/mulr_gt0.
+      + by rewrite subr_gt0; apply/FCRS.card_gt1.
+      by apply/expr_gt0/SFT.card_gt0.
+    qed.
+  
+    op n = ilog SFT.card TFT.card.
+  
+    lemma lt0n :
+      0 < n.
+    proof.
+      rewrite /n ltzE /=; move: (ilog_mono SFT.card SFT.card TFT.card).
+      rewrite ilog_b FCRS.card_gt1 SFT.card_gt0 /= => -> //.
+      by rewrite /SFT.card /TFT.card size_map size_filter count_size.
+    qed.
+  
+    lemma eq_card_pow_n :
+      TFT.card = SFT.card ^ n.
+    proof.
+      case: finite_basis_exists => vs [uniq_ basis_].
+      case: (basis_) => free_ /gen_t_enum_lin mem_e.
+      move: (free_uniq_enum_lin _ uniq_ free_) => uniq_e.
+      move: (size_enum_lin vs); rewrite /n /SFT.card /TFT.card.
+      rewrite (perm_eq_size _ TFT.enum).
+      + apply/uniq_perm_eq => // [|x]; [by apply/TFT.enum_uniq|].
+        by rewrite TFT.enumP mem_e.
+      by move=> ->; rewrite ilog_powK // FCRS.card_gt1.
+    qed.
+  end SFF.
 end SubFiniteField.
 
 
