theories/algebra/UnitRing.ec
@@ -14,60 +14,64 @@ abstract theory UZMod_ComRing.
 
   import RL.
 
-  clone import Subtype as Sub with
+  clone import Subtype as USub with
     type T  <= t,
     type sT <= uz,
     pred P  <= unit.
 
-  clone import ZModule as UZMod with
-    type t    <= uz,
-    op zeror  <= insubd oner,
-    op (+)    <= (fun x y => insubd (val x * val y)),
-    op [-]    <= (fun x => insubd (invr (val x)))
-    proof *.
+  clone include ZModuleStruct with
+    type t       <- uz,
+    op RL.zeror  <= insubd oner,
+    op RL.(+)    <= (fun x y => insubd (val x * val y)),
+    op RL.([-])  <= (fun x => insubd (invr (val x)))
+    rename [theory] "RL"      as "UZ"
+                    "ZModStr" as "UStr"
+  proof *.
 
-  realize addrA.
+  realize UZ.addrA.
   proof.
     move=> x y z; rewrite /( + ); apply/val_inj.
     rewrite !val_insubd !unitrM !valP /= !unitrM !valP /=.
     by rewrite mulrA.
   qed.
 
-  realize addrC.
+  realize UZ.addrC.
   proof.
     move=> x y; rewrite /( + ); apply/val_inj.
     rewrite !val_insubd !unitrM !valP /=.
     by rewrite mulrC.
   qed.
 
-  realize add0r.
+  realize UZ.add0r.
   proof.
     move=> x; rewrite /zeror /( + ); apply/val_inj.
     by rewrite !val_insubd unitr1 /= mul1r valP.
   qed.
 
-  realize addNr.
+  realize UZ.addNr.
   proof.
     move=> x; rewrite /zeror /( + ) /([-]); apply/val_inj; rewrite !val_insubd.
     by rewrite unitrV valP /= unitrM unitrV valP unitr1 /= mulVr // valP.
   qed.
 
   theory UZModCR.
-    import Sub.
+    import USub UZ.
 
-    lemma val1 : val UZMod.zeror = RL.oner.
+    lemma val1 : val UZ.zeror = RL.oner.
     proof. by rewrite val_insubd unitr1. qed.
 
-    lemma valM x y : val (UZMod.( + ) x y) = val x * val y.
+    lemma valM x y : val (UZ.( + ) x y) = val x * val y.
     proof. by rewrite /( + ) val_insubd unitrM !valP. qed.
 
-    lemma valV x : val (UZMod.([-]) x) = invr (val x).
-    proof. by rewrite /UZMod.([-]) val_insubd unitrV valP. qed.
+    lemma valV x : val (UZ.([-]) x) = invr (val x).
+    proof. by rewrite /UZ.([-]) val_insubd unitrV valP. qed.
 
-    lemma valXR x n :
-      0 <= n =>
-      val (UZMod.intmul x n) = exp (val x) n.
+    lemma valX x n :
+      val (UZ.intmul x n) = exp (val x) n.
     proof.
+      wlog: n / 0 <= n => [wlogn|].
+      + case (0 <= n) => [/wlogn //|] /ltrNge/ltzW/ler_opp2/=/wlogn {wlogn}.
+        by rewrite exprN mulrNz valV => /invr_inj.
       elim n => [|n le0n IHn]; [by rewrite mulr0z expr0 val1|].
       by rewrite mulrSz valM IHn exprS.
     qed.
@@ -87,8 +91,9 @@ abstract theory UZMod_IDomain.
     theory RL <- RL,
     theory ZModStr <- ZModStr,
     theory CRStr   <- CRStr
-    rename [theory] "RL"  as "Gone"
-           [theory] "Str" as "Gone".
+    rename [theory] "RL"      as "Gone"
+           [theory] "ZModStr" as "Gone"
+           [theory] "CRStr"   as "Gone".
 end UZMod_IDomain.
 
 (* -------------------------------------------------------------------- *)
@@ -99,24 +104,15 @@ abstract theory UZMod_Field.
     type t <- t.
 
   clone include UZMod_IDomain with
-    type t    <- t,
-    type uz   <- uz,
-    theory RL <- RL,
+    type t         <- t,
+    type uz        <- uz,
+    theory RL      <- RL,
     theory ZModStr <- ZModStr,
     theory CRStr   <- CRStr,
     theory IDStr   <- IDStr
     rename [theory] "RL"  as "Gone"
-           [theory] "Str" as "Gone".
-
-  theory UZModF.
-    import RL Sub UZModCR.
-    lemma valX x n :
-      val (UZMod.intmul x n) = exp (val x) n.
-    proof.
-      case (0 <= n) => [|/ltrNge/ltzW]; [by apply/valXR|].
-      rewrite -(IntID.opprK n) oppr_le0 => le0_.
-      by rewrite UZMod.mulrNz valV exprN; congr; apply/valXR.
-    qed.
-  end UZModF.
+           [theory] "ZModStr" as "Gone"
+           [theory] "CRStr"   as "Gone"
+           [theory] "IDStr"   as "UZMod_FieldIDStrGone".
 end UZMod_Field.
 
